proofs/isabelle/SpecRest/soundness/DirectSound_Smt.thy
@@ -214,6 +214,7 @@ fun smt_uses_var :: "String.literal \<Rightarrow> smt_term \<Rightarrow> bool" w
 | "smt_uses_var x (TStrLit _)            = False"
 | "smt_uses_var x (TMatches t _)         = smt_uses_var x t"
 | "smt_uses_var x (TUStrPred _ t)        = smt_uses_var x t"
+| "smt_uses_var x (TUStrFunc _ t)        = smt_uses_var x t"
 | "smt_uses_var x (TUConst _)            = False"
 | "smt_uses_var x TSeqEmpty              = False"
 | "smt_uses_var x (TSeqCons e r)         = (smt_uses_var x e \<or> smt_uses_var x r)"
